fibonacci + morse

JewelsOfStringologyLean/Fibonacci.lean
@@ -1,17 +1,20 @@
 import Mathlib.Data.Nat.Fib.Basic
 
-def FibWord (n: Nat): List Nat :=
+inductive Bin where | a : Bin | b : Bin
+open Bin
+
+def FibWord (n: Nat): List Bin :=
   match n with
   | 0 => []
-  | 1 => [1]
-  | 2 => [0]
+  | 1 => [b]
+  | 2 => [a]
   | n + 3 => FibWord (n + 2) ++ FibWord (n + 1)
 
-example : FibWord 1 = [1] := by rw [FibWord]
-example : FibWord 2 = [0] := by rw [FibWord]
-example : FibWord 3 = [0, 1] := by repeat (rw [FibWord]; repeat trivial)
-example : FibWord 4 = [0, 1, 0] := by repeat (rw [FibWord]; repeat trivial)
-example : FibWord 5 = [0, 1, 0, 0, 1] := by repeat (rw [FibWord]; repeat trivial)
+example : FibWord 1 = [b] := by rw [FibWord]
+example : FibWord 2 = [a] := by rw [FibWord]
+example : FibWord 3 = [a, b] := by repeat (rw [FibWord]; repeat trivial)
+example : FibWord 4 = [a, b, a] := by repeat (rw [FibWord]; repeat trivial)
+example : FibWord 5 = [a, b, a, a, b] := by repeat (rw [FibWord]; repeat trivial)
 
 theorem fib_word_length (n: Nat) : (FibWord n).length = Nat.fib n := by
   induction n using Nat.strong_induction_on with
