JewelsOfStringologyLean/TueMorse.lean
@@ -1,0 +1,145 @@
+import Mathlib.Tactic.SimpRw
+import Mathlib.Data.Nat.Basic
+import Mathlib.Tactic.NthRewrite
+
+variable { α : Type }
+
+inductive Bin where | a : Bin | b : Bin
+open Bin
+
+def inverseBin (x: Bin): Bin := match x with
+  | a => b
+  | b => a
+
+theorem inverse_is_involution (x: Bin) : inverseBin (inverseBin x) = x := by
+  match x with
+  | a | b => trivial
+
+def inverseWord (w: List Bin): List Bin := w.map inverseBin
+
+theorem inverseWord_is_involution (w: List Bin): inverseWord (inverseWord w) = w := by
+  induction w with
+  | nil => trivial
+  | cons h t ih =>
+    rw [inverseWord, inverseWord]
+    rw [List.map_cons, List.map_cons]
+    rw [← inverseWord, ← inverseWord]
+    simp [inverse_is_involution, ih]
+
+def TueMorseMorphism (x: Bin): List Bin := match x with
+  | a => [a, b]
+  | b => [b, a]
+
+def Morphism (m: α → List α) (w: List α) := w.flatMap m
+
+theorem morphism_distributive (m: α → List α) (w₁ w₂: List α) :
+  (Morphism m w₁) ++ (Morphism m w₂) = Morphism m (w₁ ++ w₂) := by simp [Morphism]
+
+theorem tue_morphism_inv_comm (w: List Bin) :
+  inverseWord (Morphism TueMorseMorphism w) = (Morphism TueMorseMorphism (inverseWord w)) := by
+  simp [inverseWord, inverseBin, Morphism, TueMorseMorphism]
+  simp [List.map_flatMap]
+  simp [List.flatMap_map]
+  have eq : ∀ (x: Bin), List.map inverseBin (TueMorseMorphism x) = TueMorseMorphism (inverseBin x) := by
+    intro x
+    match x with
+    | a | b => trivial
+  simp_rw [eq]
+
+theorem morphism_const_length (m: α → List α) (l: Nat) (hl: ∀ (x: α), (m x).length = l) (w: List α) :
+  (Morphism m w).length = w.length * l := by
+  simp [Morphism]
+  conv in (m _).length => apply hl
+  induction w with
+  | nil => simp
+  | cons h t ih => simp +arith [ih, Nat.add_mul]
+
+example : Morphism TueMorseMorphism (Morphism TueMorseMorphism [a]) = [a, b, b, a] := by trivial
+
+def TueMorseWord (n: Nat): List Bin := match n with
+  | 0 => [a]
+  | n + 1 => Morphism TueMorseMorphism (TueMorseWord (n))
+
+def TueMorseWordAlt (n: Nat): List Bin := match n with
+  | 0 => [a]
+  | n + 1 => (TueMorseWordAlt n) ++ inverseWord (TueMorseWordAlt n)
+
+example : TueMorseWord 3 = [a, b, b, a, b, a, a, b] := by
+  simp [TueMorseWord, Morphism, TueMorseMorphism, List.flatMap_eq_foldl]
+
+example : TueMorseWordAlt 3 = [a, b, b, a, b, a, a, b] := by
+  simp [TueMorseWordAlt, inverseWord, inverseBin]
+
+theorem tue_morse_morphism_length (x: Bin) : (TueMorseMorphism x).length = 2 := by
+  match x with
+  | a | b => trivial
+
+theorem tue_morse_word_length (n: Nat): (TueMorseWord n).length = 2^n := by
+  induction n with
+  | zero => trivial
+  | succ n ih =>
+    rw [TueMorseWord]
+    rw [morphism_const_length TueMorseMorphism 2 tue_morse_morphism_length (TueMorseWord n)]
+    omega
+
+theorem tue_morse_word_alt_length (n: Nat): (TueMorseWordAlt n).length = 2^n := by
+  induction n with
+  | zero => trivial
+  | succ n ih =>
+    rw [TueMorseWordAlt]
+    simp [ih, inverseWord]
+    omega
+
+theorem tue_morse_def_eq (n: Nat) : TueMorseWord n = TueMorseWordAlt n := by
+  induction n using Nat.strong_induction_on with
+  | h n ih => match n with
+    | 0 | 1 => trivial
+    | n + 2 =>
+      let x := TueMorseWord (n + 1)
+      let x_l := x.take (2^n)
+      let x_r := x.drop (2^n)
+
+      let y := TueMorseWordAlt (n + 1)
+      let y_l := y.take (2^n)
+      let y_r := y.drop (2^n)
+
+      have x_l_eq_y_l : x_l = y_l := by simp [x_l, y_l, x, y, ih]
+      have x_r_eq_y_r : x_r = y_r := by simp [x_r, y_r, x, y, ih]
+
+      have y_l_eq_tn : y_l = TueMorseWordAlt n := by
+        simp only [y, y_l, TueMorseWordAlt]
+        rw [List.take_append_of_le_length, List.take_of_length_le]
+        repeat rw [tue_morse_word_alt_length]
+
+      have : y_r = inverseWord (TueMorseWordAlt n) := by
+        simp only [y, y_r, TueMorseWordAlt]
+        rw [List.drop_append_of_le_length, List.drop_of_length_le]
+        simp
+        repeat rw [tue_morse_word_alt_length]
+
+      have : y_l ++ inverseWord y_l = y := by simp_all only [y, y_l, TueMorseWordAlt]
+      have : y_l ++ y_r = y := by simp_all only
+      have y_r_eq_not_y_l : y_r = inverseWord y_l := by simp_all [inverseWord_is_involution]
+
+      have y_l_morph : (Morphism TueMorseMorphism y_l) = TueMorseWordAlt (n + 1) := by
+        rw [← x_l_eq_y_l]
+        rw [← ih]
+        rw [TueMorseWord]
+        rw [x_l_eq_y_l, y_l_eq_tn]
+        rw [ih]
+        repeat simp
+
+      have x_break : (Morphism TueMorseMorphism x_l) ++ (Morphism TueMorseMorphism x_r) =
+              Morphism TueMorseMorphism x := by
+        simp only [morphism_distributive, x_l, x_r, List.take_append_drop]
+
+      rw [TueMorseWord]
+      rw [← x_break]
+      rw [x_l_eq_y_l, x_r_eq_y_r]
+      rw [y_r_eq_not_y_l]
+      rw [← tue_morphism_inv_comm]
+      rw [y_l_morph]
+      rw [← ih]
+      rw [TueMorseWordAlt]
+      rw [ih]
+      repeat simp
